Femto_VHDL_Executable.thy
@@ -5,12 +5,11 @@
  * the BSD 2-Clause license. Note that NO WARRANTY is provided.
  * See "LICENSE_BSD2.txt" for details.
  *
- *  Author: Albert Rizaldi, NTU Singapore 
+ *  Author: Albert Rizaldi, NTU Singapore
  *)
 
 theory Femto_VHDL_Executable
   imports Femto_VHDL
-          "Polynomials.Poly_Mapping_Finite_Map"
 begin
 
 datatype sig = A | B | C
@@ -47,6 +46,14 @@ lemma zero_upd:
   "0 (sig := None) = 0"
   by (auto simp add:zero_map zero_option_def)
 
+definition to_transaction2' :: "'signal transaction \<Rightarrow> 'signal transaction2" where
+  "to_transaction2' \<tau> = (\<lambda>s. Poly_Mapping.map (\<lambda>m. m s) \<tau>)"
+
+lemma [code]:
+  "to_transaction2 \<tau> = to_transaction2' \<tau>"
+  unfolding to_transaction2'_def
+  by (transfer', unfold to_trans_raw2_def)(metis (mono_tags, hide_lams) "when"(1) when_def zero_fun_def)
+
 value [code] "signals_in (Bassign_trans C Btrue 0)"
 value [code] "beval 0 def_state {} 0 (Bsig A)"
 value [code] "beval 0 def_state {} 0 (Band (Bsig A) (Bsig B))"
@@ -56,7 +63,7 @@ definition
 
 lemma lookup0_fmdrop:
   "lookup0 (fmdrop x xa) = map_drop x (lookup0 xa)"
-  by (auto simp add: fmlookup_default_def Finite_Map.map_filter_def map_drop_def zero_option_def  
+  by (auto simp add: fmlookup_default_def Finite_Map.map_filter_def map_drop_def zero_option_def
               split: option.splits)
 
 lemma lookup0_fmupd:
@@ -65,7 +72,7 @@ lemma lookup0_fmupd:
 
 (* TODO : streamline this proof; applying auto in the middle is ugly *)
 lemma lookup0_update_with_none:
-  "(lookup0 xs)(time := (lookup0 xs time)(sig := None)) = 
+  "(lookup0 xs)(time := (lookup0 xs time)(sig := None)) =
     lookup0 (fmupd time (map_drop sig (lookup0 xs time)) xs)"
   apply (auto simp add: fmlookup_default_def Finite_Map.map_filter_def map_drop_def zero_option_def
               split: option.splits)
@@ -73,13 +80,13 @@ lemma lookup0_update_with_none:
 proof (rule_tac[!] ext)
   fix a'
   assume "fmlookup xs time = None"
-  thus "((lookup0 xs)(time := 0(sig := None))) a' = 
+  thus "((lookup0 xs)(time := 0(sig := None))) a' =
             (if time = a' then \<lambda>x. if x \<noteq> sig then 0 x else None else lookup0 xs a')"
     by auto
 next
   fix x2 a'
   assume "fmlookup xs time = Some x2"
-  thus "((lookup0 xs)(time := x2(sig := None))) a' = 
+  thus "((lookup0 xs)(time := x2(sig := None))) a' =
             (if time = a' then \<lambda>x. if x \<noteq> sig then x2 x else None else lookup0 xs a')"
     by auto
 qed
@@ -89,26 +96,26 @@ lemma [code]:
   by (transfer, auto)
 
 lemma [code]:
-  "purge (Suc n) (Pm_fmap xs) now sig val = 
+  "purge (Suc n) (Pm_fmap xs) now sig val =
       (let f   = lookup0 xs (now + Suc n);
            f'  = map_drop sig f;
-           xs' = fmupd (now + Suc n) f' xs 
-       in 
-          if f sig = Some val then purge n (Pm_fmap xs) now sig val 
+           xs' = fmupd (now + Suc n) f' xs
+       in
+          if f sig = Some val then purge n (Pm_fmap xs) now sig val
           else purge n (Pm_fmap xs') now sig val)"
-  by (transfer, auto simp add: lookup0_update_with_none Let_def) 
- 
+  by (transfer, auto simp add: lookup0_update_with_none Let_def)
+
 value "lookup (purge 1 (0 :: sig transaction) 1 C True) 1 C"
 
 lemma [code]:
-  "trans_post sig v (Pm_fmap xs) t = (let 
+  "trans_post sig v (Pm_fmap xs) t = (let
                                           current = lookup0 xs t;
                                           chopped = fmmap_keys (\<lambda>t'. if t < t' then map_drop sig else id);
-                                          updated = fmupd t (current(sig \<mapsto> v)) xs  
-                                      in 
+                                          updated = fmupd t (current(sig \<mapsto> v)) xs
+                                      in
                                           Pm_fmap (chopped updated))"
   by (transfer', unfold Let_def trans_post_raw_def)
-     (rule ext, auto simp add: fmlookup_default_def zero_map map_drop_def map_filter_def 
+     (rule ext, auto simp add: fmlookup_default_def zero_map map_drop_def map_filter_def
                         split: option.splits)
 
 value [code] "beval 2 def_state {} test_beh (Bsig_delayed A 1)"
@@ -125,30 +132,30 @@ definition
 definition
   "exp3 = Bnot (Bor (Bsig C) (Bsig B))"
 
-definition 
+definition
   "seq1 = Bassign_trans C exp2 1"
 
 definition
   "seq2 = Bassign_inert B exp3 2"
 
-definition                                                                
-  "seq3 = Bguarded exp1 seq1 seq2"          
+definition
+  "seq3 = Bguarded exp1 seq1 seq2"
 
 value [code] "lookup (b_seq_exec 0 def_state {} 0 (Bcomp seq1 seq2) empty_trans) 1 C"
 value [code] "lookup (b_seq_exec 0 def_state {} 0 (Bguarded exp1 seq1 seq2) empty_trans) 2 C"
 value [code] "lookup (b_seq_exec 0 def_state {} 0 seq1 empty_trans) 1 C"
-value [code] "lookup (b_seq_exec 0 def_state {} 0 seq2 empty_trans) 2 C" 
+value [code] "lookup (b_seq_exec 0 def_state {} 0 seq2 empty_trans) 2 C"
 
 
 term "fmmap_keys (\<lambda>x. fmadd)"
 
 lemma [code]:
-  "map_add_trans (Pm_fmap xs) (Pm_fmap ys) =  
+  "map_add_trans (Pm_fmap xs) (Pm_fmap ys) =
                                Pm_fmap (fmmap_keys (\<lambda>k v. lookup0 xs k ++ lookup0 ys k) (xs ++\<^sub>f ys))"
   by (transfer') (rule ext, auto simp add:fmlookup_default_def map_add_subsumed1 split:option.splits)
 
 lemma [code]:
-  "map_diff_trans (Pm_fmap xs) (Pm_fmap ys) = 
+  "map_diff_trans (Pm_fmap xs) (Pm_fmap ys) =
                      Pm_fmap (fmmap_keys (\<lambda>k v. map_diff (lookup0 xs k) (lookup0 ys k)) (xs ++\<^sub>f ys))"
   by (transfer') (rule ext, auto simp add: fmlookup_default_def zero_map split:option.splits)
 
@@ -156,7 +163,7 @@ lemma clean_zip_alt_def [code]:
   "clean_zip \<tau> \<tau>1 \<tau>2 = (let \<tau>1_stripped = map_diff_trans \<tau>1 \<tau>;
                            \<tau>2_stripped = map_diff_trans \<tau>2 \<tau>;
                            zipped = map_add_trans \<tau>1_stripped \<tau>2_stripped
-                        in 
+                        in
                            map_add_trans \<tau> zipped)"
   by (transfer) (auto simp add:clean_zip_raw_def)
 
@@ -166,7 +173,7 @@ value [code] "lookup (b_conc_exec 1 def_state {A, B} test_beh (process {A} : seq
 value [code] "lookup (b_conc_exec 1 def_state {A, C} test_beh ((process {A} : seq1) || (process {C} : seq2)) empty_trans) 3 B"
 
 value [code] "quiet (empty_trans :: sig transaction) {}"
-                  
+
 
 lemma [code]:
   "Poly_Mapping.update k v (Pm_fmap xs) = Pm_fmap (fmupd k v xs)"
@@ -176,8 +183,8 @@ value [code] "rem_curr_trans 0 (empty_trans :: sig transaction)"
 
 
 lemma lookup0_zero_fun:
-  "lookup0 xs = (\<lambda>k. 0) \<longleftrightarrow> clearjunk0 xs = fmempty" 
-  by (metis PM_clearjunk0_cong Pm_fmap.rep_eq aux compute_keys_pp compute_zero_pp 
+  "lookup0 xs = (\<lambda>k. 0) \<longleftrightarrow> clearjunk0 xs = fmempty"
+  by (metis PM_clearjunk0_cong Pm_fmap.rep_eq aux compute_keys_pp compute_zero_pp
             fmap_exhaust fmdom'_fmupd insert_iff lookup_not_eq_zero_eq_in_keys)
 
 lemma LEAST_ext:
@@ -215,19 +222,19 @@ proof -
     by (auto simp add: sorted_list_of_fset.rep_eq)
   also have "... = insort x (sorted_list_of_fset (fmdom (fmdrop x m)))"
     by auto
-  finally show "sorted_list_of_fset (fmdom (fmupd x y m)) = 
+  finally show "sorted_list_of_fset (fmdom (fmupd x y m)) =
                    insort x (sorted_list_of_fset (fmdom (fmdrop x m)))"
     by auto
 qed
 
 lemma sorted_list_of_fmap_fmupd:
-  "sorted_list_of_fmap (fmupd x y m) = 
+  "sorted_list_of_fmap (fmupd x y m) =
    map (\<lambda>k. (k, the (fmlookup (fmupd x y m) k))) (insort x (sorted_list_of_fset (fmdom (fmdrop x m))))"
-proof -               
-  have "sorted_list_of_fset (fmdom (fmupd x y m)) = 
+proof -
+  have "sorted_list_of_fset (fmdom (fmupd x y m)) =
                    insort x (sorted_list_of_fset (fmdom (fmdrop x m)))"
     using sorted_list_fmdom_fmupd by auto
-  thus "sorted_list_of_fmap (fmupd x y m) = 
+  thus "sorted_list_of_fmap (fmupd x y m) =
     map (\<lambda>k. (k, the (fmlookup (fmupd x y m) k))) (insort x (sorted_list_of_fset (fmdom (fmdrop x m))))"
     unfolding sorted_list_of_fmap_def by auto
 qed
@@ -248,8 +255,8 @@ proof -
     "\<forall>f fa. fa = f \<or> map_of (sorted_list_of_fmap fa) (aa fa f) \<noteq> map_of (sorted_list_of_fmap f) (aa fa f)"
     by (metis fmap_ext map_of_sorted_list)
   then have " fst (hd (sorted_list_of_fmap m)) = hd (map fst (sorted_list_of_fmap m))"
-    using a1 by (metis (no_types) bot_fset.rep_eq fmdom_empty list.map_sel(1) list.simps(8) 
-                 map_of_sorted_list sorted_list_of_fmap_def sorted_list_of_fset.rep_eq 
+    using a1 by (metis (no_types) bot_fset.rep_eq fmdom_empty list.map_sel(1) list.simps(8)
+                 map_of_sorted_list sorted_list_of_fmap_def sorted_list_of_fset.rep_eq
                  sorted_list_of_set_empty)
   also have "... = hd (sorted_list_of_fset (fmdom m))"
     unfolding sorted_list_of_fmap_def by (simp add: o_def)
@@ -277,7 +284,7 @@ proof -
     using `fmlookup (clearjunk0 m) k = Some val` unfolding fmlookup_default_def
     by auto
   hence "lookup0 m k \<noteq> Map.empty"
-    unfolding clearjunk0_def 
+    unfolding clearjunk0_def
     by (metis \<open>lookup0 (clearjunk0 m) k \<noteq> Map.empty\<close> lookup0_clearjunk0)
   thus ?thesis
     by (intro exI[where x="k"])
@@ -307,26 +314,26 @@ proof (induction xs rule: fmap_induct)
   then show ?case by (auto simp add: clearjunk0_def)
 next
   case (fmupd x y m)
-  have "clearjunk0 m = fmempty \<or> clearjunk0 m \<noteq> fmempty" 
+  have "clearjunk0 m = fmempty \<or> clearjunk0 m \<noteq> fmempty"
     by auto
   moreover
   { assume *: "clearjunk0 m = fmempty"
     have "(LEAST n. lookup0 (fmupd x y m) n \<noteq> Map.empty) = x"
-    proof (rule Least_equality) 
+    proof (rule Least_equality)
       have **: "x \<in> fmdom' (clearjunk0 (fmupd x y m))"
-        using fmupd(3) *  by (metis (mono_tags, hide_lams) compute_keys_pp compute_lookup_pp 
+        using fmupd(3) *  by (metis (mono_tags, hide_lams) compute_keys_pp compute_lookup_pp
                                     in_keys_iff  lookup0_fmupd lookup0_zero_fun)
       have " lookup0 (fmupd x y m) x = lookup0 (clearjunk0 (fmupd x y m)) x"
         using lookup0_clearjunk0 by metis
       moreover have "... \<noteq> Map.empty"
-        using fmupd(3) 
+        using fmupd(3)
         apply (auto simp add:fmlookup_default_def split:option.splits)
         apply (metis "*"calculation fmlookup_default_if(2) lookup0_fmupd lookup0_zero_fun)
         using clearjunk0_nonzero[OF **] zero_fun_def zero_option_def
-        by (metis "**" PM_clearjunk0_cong calculation clearjunk0_map_of_SomeD clearjunk0_nonzero 
+        by (metis "**" PM_clearjunk0_cong calculation clearjunk0_map_of_SomeD clearjunk0_nonzero
                        compute_keys_pp ext fmlookup_default_def fmupd_lookup option.simps(5))
       ultimately show "lookup0 (fmupd x y m) x \<noteq> Map.empty"
-        by auto 
+        by auto
     next
       { fix ya
         assume "\<not> x \<le> ya" hence "ya <  x" by auto
@@ -350,7 +357,7 @@ next
         using * by auto
       finally have "fmdom (clearjunk0 (fmupd x y m)) =  {|x|}"
         by auto
-      moreover have "the (fmlookup (clearjunk0 (fmupd x y m)) x) = y"        
+      moreover have "the (fmlookup (clearjunk0 (fmupd x y m)) x) = y"
       proof -
         have "fmlookup (fmupd x y m) x \<noteq> Some 0"
           using \<open>fmlookup (fmupd x y m) x \<noteq> Some 0\<close> by blast
@@ -369,16 +376,16 @@ next
       by auto
     obtain cur_least where cur_least_def: "cur_least = (LEAST n. lookup0 m n \<noteq> Map.empty) "
       by auto
-    consider (new) "x < cur_least" | (old) "cur_least \<le> x" 
+    consider (new) "x < cur_least" | (old) "cur_least \<le> x"
       using le_less_linear by blast
-    hence ?case 
+    hence ?case
     proof (cases)
       case new
       have "lookup0 (fmupd x y m) x = Map.empty \<or> lookup0 (fmupd x y m) x \<noteq> Map.empty"
         by auto
       moreover
       { assume "lookup0 (fmupd x y m) x = Map.empty"
-        hence "(LEAST n. lookup0 (fmupd x y m) n \<noteq> Map.empty) = 
+        hence "(LEAST n. lookup0 (fmupd x y m) n \<noteq> Map.empty) =
                (LEAST n. n \<noteq> x \<and> lookup0 (fmupd x y m) n \<noteq> Map.empty)"
           by metis
         also have "... = (LEAST n. lookup0 m n \<noteq> Map.empty)"
@@ -390,19 +397,19 @@ next
                                                       fst (hd (sorted_list_of_fmap (clearjunk0 m)))"
           by auto
         have "y = 0"
-          using `lookup0 (fmupd x y m) x = Map.empty` 
+          using `lookup0 (fmupd x y m) x = Map.empty`
           by (auto simp add:zero_map)
-        have "clearjunk0 (fmupd x y m) = fmdrop x (clearjunk0 m)"  
+        have "clearjunk0 (fmupd x y m) = fmdrop x (clearjunk0 m)"
           using clearjunk0_fmupd_with_0 unfolding `y = 0` by metis
         also have "... = clearjunk0 m"
           using fmupd(2)  by (simp add: clearjunk0_def fmap_ext)
         finally have "clearjunk0 (fmupd x y m) = clearjunk0 m"
           by auto
-        hence "fst (hd (sorted_list_of_fmap (clearjunk0 (fmupd x y m)))) = 
+        hence "fst (hd (sorted_list_of_fmap (clearjunk0 (fmupd x y m)))) =
                                                       fst (hd (sorted_list_of_fmap (clearjunk0 m)))"
           by auto
         with lexpand have ?thesis by auto }
-      moreover 
+      moreover
       { assume "lookup0 (fmupd x y m) x \<noteq> Map.empty"
         hence "y \<noteq> Map.empty" by auto
         have lexpand2: "(LEAST n. lookup0 (fmupd x y m) n \<noteq> Map.empty) = x"
@@ -417,7 +424,7 @@ next
             have "ya < cur_least"
               using `ya < x` and `x < cur_least` by auto
             hence "lookup0 m ya = Map.empty"
-              unfolding cur_least_def using not_less_Least by auto 
+              unfolding cur_least_def using not_less_Least by auto
             hence "lookup0 (fmupd x y m) ya = Map.empty"
               using `lookup0 (fmupd x y m) ya = lookup0 m ya` by auto }
           thus "\<And>ya. lookup0 (fmupd x y m) ya \<noteq> Map.empty \<Longrightarrow> x \<le> ya "
@@ -425,30 +432,30 @@ next
         qed
         have push_clearjunk0: "clearjunk0 (fmupd x y m) = fmupd x y (clearjunk0 m)"
           by (metis \<open>y \<noteq> Map.empty\<close> clearjunk0_fmupd_neq_0 zero_map)
-        hence swap_cj_fmupd: "sorted_list_of_fmap (clearjunk0 (fmupd x y m)) = 
+        hence swap_cj_fmupd: "sorted_list_of_fmap (clearjunk0 (fmupd x y m)) =
                sorted_list_of_fmap (fmupd x y (clearjunk0 m))"
           by auto
-        have "... = 
-            map (\<lambda>k. (k, the (fmlookup (fmupd x y (clearjunk0 m)) k))) 
+        have "... =
+            map (\<lambda>k. (k, the (fmlookup (fmupd x y (clearjunk0 m)) k)))
                                               (insort x (sorted_list_of_fset (fmdom (fmdrop x (clearjunk0 m)))))"
             (is "?simple = ?complex")
           using sorted_list_of_fmap_fmupd by auto
         have "fmdrop x (clearjunk0 m) = clearjunk0 m"
           by (simp add: fmupd clearjunk0_def fmap_ext)
-        hence "sorted_list_of_fset (fmdom (fmdrop x (clearjunk0 m))) = 
+        hence "sorted_list_of_fset (fmdom (fmdrop x (clearjunk0 m))) =
                sorted_list_of_fset (fmdom (clearjunk0 m))"
           by auto
-        moreover have "insort x (sorted_list_of_fset (fmdom (clearjunk0 m))) = 
+        moreover have "insort x (sorted_list_of_fset (fmdom (clearjunk0 m))) =
             x # (sorted_list_of_fset (fmdom (clearjunk0 m)))"
-          using new unfolding cur_least_def 
+          using new unfolding cur_least_def
           using ind  unfolding dom_only[OF `clearjunk0 m \<noteq> fmempty`]
           by (metis (no_types, lifting) insort_key.simps(1) insort_key.simps(2) less_imp_le list.collapse)
-        ultimately have x_as_hd: "insort x (sorted_list_of_fset (fmdom (fmdrop x (clearjunk0 m)))) = 
+        ultimately have x_as_hd: "insort x (sorted_list_of_fset (fmdom (fmdrop x (clearjunk0 m)))) =
                x # sorted_list_of_fset (fmdom (clearjunk0 m))"
-          by auto      
+          by auto
         have "fst (hd (sorted_list_of_fmap (clearjunk0 (fmupd x y m)))) =  x"
           using swap_cj_fmupd `?simple = ?complex` x_as_hd by auto
-        with lexpand2 have ?thesis by auto }    
+        with lexpand2 have ?thesis by auto }
       ultimately show ?thesis by auto
     next
       case old
@@ -456,12 +463,12 @@ next
       proof (rule ccontr)
         assume "\<not> x \<noteq> cur_least"
         hence "x = cur_least" by auto
-        obtain k where k_not_emp: "lookup0 m k \<noteq> Map.empty" 
+        obtain k where k_not_emp: "lookup0 m k \<noteq> Map.empty"
           using `clearjunk0 m \<noteq> fmempty`
-          by (smt Pm_fmap.rep_eq clearjunk0_def compute_keys_pp fmdom'_filter fmdom'_notI 
+          by (smt Pm_fmap.rep_eq clearjunk0_def compute_keys_pp fmdom'_filter fmdom'_notI
                   fmfilter_false fmlookup_default_if(1) fmupd(2) in_keys_iff member_filter)
         hence "lookup0 m x \<noteq> Map.empty"
-          using LeastI[where P = "\<lambda>x. lookup0 m x \<noteq> Map.empty", OF k_not_emp] `x = cur_least` 
+          using LeastI[where P = "\<lambda>x. lookup0 m x \<noteq> Map.empty", OF k_not_emp] `x = cur_least`
           unfolding cur_least_def by auto
         thus "False"
           using fmupd(2) by (simp add: zero_fun_def zero_option_def)
@@ -491,7 +498,7 @@ next
         thus "\<And>ya. lookup0 (fmupd x y m) ya \<noteq> Map.empty \<Longrightarrow> cur_least \<le> ya "
           by blast
       qed
-      have fi_rexpand: "fst (hd (sorted_list_of_fmap (clearjunk0 (fmupd x y m)))) = 
+      have fi_rexpand: "fst (hd (sorted_list_of_fmap (clearjunk0 (fmupd x y m)))) =
             hd (sorted_list_of_fset (fmdom (clearjunk0 (fmupd x y m))))"
         using dom_only[OF `clearjunk0 (fmupd x y m) \<noteq> fmempty`] by auto
 
@@ -501,7 +508,7 @@ next
         hence "clearjunk0 (fmupd x y m) = fmdrop x (clearjunk0 m)"
           using clearjunk0_fmupd_with_0[of "x" "m"]  by (simp add: zero_fun_def zero_option_def)
         also have "... = clearjunk0 m"
-          using fmupd(2)  by (simp add: clearjunk0_def fmap_ext) 
+          using fmupd(2)  by (simp add: clearjunk0_def fmap_ext)
         finally have "clearjunk0 (fmupd x y m) = clearjunk0 m"
           by auto
         hence " hd (sorted_list_of_fset (fmdom (clearjunk0 (fmupd x y m)))) =
@@ -514,17 +521,17 @@ next
           using fi_rexpand by auto
         also have "... = cur_least"
           using ind unfolding cur_least_def by auto
-        finally have "fst (hd (sorted_list_of_fmap (clearjunk0 (fmupd x y m)))) = 
+        finally have "fst (hd (sorted_list_of_fmap (clearjunk0 (fmupd x y m)))) =
                       cur_least" by auto
         with lexpand_old have ?thesis by auto }
-    
+
       moreover
       { assume "y \<noteq> Map.empty"
         have push_clearjunk0_old: "clearjunk0 (fmupd x y m) = fmupd x y (clearjunk0 m)"
           by (metis \<open>y \<noteq> Map.empty\<close> clearjunk0_fmupd_neq_0 zero_map)
         hence fmdom_clearjunk: "fmdom (clearjunk0 (fmupd x y m)) = fmdom (fmupd x y (clearjunk0 m))"
           by auto
-        have "sorted_list_of_fset (fmdom (fmupd x y (clearjunk0 m))) = 
+        have "sorted_list_of_fset (fmdom (fmupd x y (clearjunk0 m))) =
               insort x (sorted_list_of_fset (fmdom (fmdrop x (clearjunk0  m)))) "
           using sorted_list_fmdom_fmupd by auto
         moreover have "fmdrop x (clearjunk0 m) = clearjunk0 m"
@@ -532,14 +539,14 @@ next
         ultimately have ****: "sorted_list_of_fset (fmdom (fmupd x y (clearjunk0 m))) =
                       insort x (sorted_list_of_fset (fmdom (clearjunk0  m)))"
           by auto
-        hence "sorted_list_of_fset (fmdom (clearjunk0 (fmupd x y m))) = 
+        hence "sorted_list_of_fset (fmdom (clearjunk0 (fmupd x y m))) =
                insort x (sorted_list_of_fset (fmdom (clearjunk0 m)))"
           using push_clearjunk0_old by auto
-        have "hd (insort x (sorted_list_of_fset (fmdom (clearjunk0 m)))) = 
+        have "hd (insort x (sorted_list_of_fset (fmdom (clearjunk0 m)))) =
                         hd (sorted_list_of_fset (fmdom (clearjunk0 m)))"
         proof (rule hd_after_insert_larger_key)
           show "sorted_list_of_fset (fmdom (clearjunk0 m)) \<noteq> []"
-            by (metis \<open>clearjunk0 m \<noteq> fmempty\<close> fmrestrict_fset_dom fmrestrict_fset_null fset_of_list_simps(1) 
+            by (metis \<open>clearjunk0 m \<noteq> fmempty\<close> fmrestrict_fset_dom fmrestrict_fset_null fset_of_list_simps(1)
                       sorted_list_of_fset_simps(2))
         next
           show " hd (sorted_list_of_fset (fmdom (clearjunk0 m))) < x "
@@ -551,7 +558,7 @@ next
           using ind unfolding cur_least_def by auto
         finally have "hd (insort x (sorted_list_of_fset (fmdom (clearjunk0 m)))) =
                          cur_least" by auto
-        hence "fst (hd (sorted_list_of_fmap (clearjunk0 (fmupd x y m)))) = 
+        hence "fst (hd (sorted_list_of_fmap (clearjunk0 (fmupd x y m)))) =
                 cur_least"
           using  **** fi_rexpand push_clearjunk0_old by auto
         with lexpand_old have ?thesis by auto }
@@ -562,8 +569,8 @@ qed
 
 lemma [code]:
   "next_time t (Pm_fmap xs) = (if clearjunk0 xs = fmempty then t else (fst o hd) (sorted_list_of_fmap (clearjunk0 xs)))"
-  unfolding next_time_def 
-  by (transfer', auto simp add: least_fst_hd_sorted lookup0_zero_fun) 
+  unfolding next_time_def
+  by (transfer', auto simp add: least_fst_hd_sorted lookup0_zero_fun)
 
 value [code] "next_time 0 (empty_trans :: sig transaction)"
 value [code] "next_state 0 (empty_trans :: sig transaction) def_state B"
@@ -575,13 +582,13 @@ definition fm_const_interval_open_right :: "'a :: zero \<Rightarrow> nat \<Right
 lemma fmlookup_const_interval_if:
   "x \<in> {lo ..< hi} \<Longrightarrow> fmlookup (fm_const_interval_open_right v lo hi) x = Some v"
   "x \<notin> {lo ..< hi} \<Longrightarrow> fmlookup (fm_const_interval_open_right v lo hi) x = None"
-  unfolding fm_const_interval_open_right_def fmlookup_of_list 
-  by (metis distinct_upt in_set_impl_in_set_zip1 in_set_replicate length_replicate length_upt 
+  unfolding fm_const_interval_open_right_def fmlookup_of_list
+  by (metis distinct_upt in_set_impl_in_set_zip1 in_set_replicate length_replicate length_upt
             map_fst_zip map_of_eq_Some_iff set_upt set_zip_rightD) (auto)
 
 
 lemma [code]:
-  "override_lookups_on_open_right (Pm_fmap xs) v lo hi = 
+  "override_lookups_on_open_right (Pm_fmap xs) v lo hi =
                                               Pm_fmap (xs  ++\<^sub>f fm_const_interval_open_right v lo hi)"
 proof (transfer', rule ext)
   fix x lo hi :: nat
@@ -596,8 +603,8 @@ proof (transfer', rule ext)
     hence "override_on (lookup0 xs) (\<lambda>n. v) {lo..<hi} x = v"
       unfolding override_on_def by auto
     moreover have "lookup0 (xs ++\<^sub>f fm_const_interval_open_right v lo hi) x = v"
-      by (metis \<open>x \<in> {lo..<hi}\<close> fmlookup_add fmlookup_const_interval_if(1) fmlookup_default_if(1) 
-                fmlookup_dom_iff)  
+      by (metis \<open>x \<in> {lo..<hi}\<close> fmlookup_add fmlookup_const_interval_if(1) fmlookup_default_if(1)
+                fmlookup_dom_iff)
     ultimately have "?le = ?ri"
       by auto }
   moreover
@@ -605,22 +612,22 @@ proof (transfer', rule ext)
     hence "override_on (lookup0 xs) (\<lambda>n. v) {lo..<hi} x = lookup0 xs x"
       unfolding override_on_def by auto
     moreover have "lookup0 (xs ++\<^sub>f fm_const_interval_open_right v lo hi) x = lookup0 xs x"
-      by (metis \<open>x \<notin> {lo..<hi}\<close> fmlookup_const_interval_if(2) fmlookup_default_add fmlookup_dom_iff 
+      by (metis \<open>x \<notin> {lo..<hi}\<close> fmlookup_const_interval_if(2) fmlookup_default_add fmlookup_dom_iff
                 option.simps(3))
     ultimately have "?le = ?ri"
       by auto }
   ultimately show "?le = ?ri"
     by blast
 qed
-            
-value [code] "add_to_beh (def_state :: sig state) {A, B, C}" 
+
+value [code] "add_to_beh (def_state :: sig state) {A, B, C}"
 
 code_thms add_to_beh
 
 code_thms next_event
 
 definition next_event_code :: "time \<Rightarrow> 'signal transaction \<Rightarrow> 'signal state \<Rightarrow> 'signal event" where
-  "next_event_code t \<tau>' \<sigma> = (let m = get_trans \<tau>' (next_time t \<tau>') in  
+  "next_event_code t \<tau>' \<sigma> = (let m = get_trans \<tau>' (next_time t \<tau>') in
                                        {sig. if sig \<in> dom m then (the o m) sig \<noteq> \<sigma> sig else False})"
 
 lemma [code]:
@@ -633,7 +640,7 @@ code_pred (modes : i \<Rightarrow> i \<Rightarrow> i \<Rightarrow> i \<Rightarro
 
 thm b_simulate_fin.equation
 
-definition "functional_simulate_fin maxtime t \<sigma> \<gamma> \<theta> cs \<tau> = 
+definition "functional_simulate_fin maxtime t \<sigma> \<gamma> \<theta> cs \<tau> =
             Predicate.the (b_simulate_fin_i_i_i_i_i_i_i_o maxtime t \<sigma> \<gamma> \<theta> cs \<tau>)"
 
 theorem functional_simulate_fin_complete:
@@ -650,9 +657,9 @@ qed
 
 code_pred (modes : i \<Rightarrow> i \<Rightarrow> o \<Rightarrow> bool) b_simulate .
 
-lemma functional_simulate_fin_sound:                      
+lemma functional_simulate_fin_sound:
   assumes "simulate_ss maxtime cs (\<tau>, t, \<sigma>, \<gamma>, \<theta>) (\<tau>', maxtime + 1, \<sigma>', \<gamma>', \<theta>')"
-  assumes "\<forall>n. t \<le> n \<longrightarrow> Poly_Mapping.lookup \<theta> n = 0" 
+  assumes "\<forall>n. t \<le> n \<longrightarrow> Poly_Mapping.lookup \<theta> n = 0"
   assumes "\<forall>n. n < t \<longrightarrow> get_trans \<tau> n = 0"
   assumes "functional_simulate_fin maxtime t \<sigma> \<gamma> \<theta> cs \<tau> = beh"
   shows "b_simulate_fin maxtime t \<sigma> \<gamma> \<theta> cs \<tau> beh"
@@ -666,24 +673,24 @@ proof -
     using assms(1) by auto
   have **: "b_simulate_fin maxtime t \<sigma> \<gamma> \<theta> cs \<tau> (Poly_Mapping.update (maxtime + 1) 0 \<theta>')"
     using small_step_implies_big_step[OF ss assms(2) assms(3)] by auto
-  hence "\<And>beh. b_simulate_fin maxtime t \<sigma> \<gamma> \<theta> cs \<tau> beh \<Longrightarrow> 
+  hence "\<And>beh. b_simulate_fin maxtime t \<sigma> \<gamma> \<theta> cs \<tau> beh \<Longrightarrow>
                                                beh = (Poly_Mapping.update (maxtime + 1) 0 \<theta>')"
     by (simp add: b_simulate_fin_deterministic)
   from * show "b_simulate_fin maxtime t \<sigma> \<gamma> \<theta> cs \<tau> beh"
-    by (metis ** b_simulate_fin_deterministic theI)  
+    by (metis ** b_simulate_fin_deterministic theI)
 qed
 
 lemma functional_simulate_eq_b_simulate_fin:
   assumes "simulate_ss maxtime cs (\<tau>, t, \<sigma>, \<gamma>, \<theta>) (\<tau>', maxtime + 1, \<sigma>', \<gamma>', \<theta>')"
-  assumes "\<forall>n. t  \<le> n \<longrightarrow> Poly_Mapping.lookup \<theta> n = 0"  
+  assumes "\<forall>n. t  \<le> n \<longrightarrow> Poly_Mapping.lookup \<theta> n = 0"
   assumes "\<forall>n. n < t \<longrightarrow> get_trans \<tau> n = 0"
   shows "b_simulate_fin maxtime t \<sigma> \<gamma> \<theta> cs \<tau> beh \<longleftrightarrow> (functional_simulate_fin maxtime t \<sigma> \<gamma> \<theta> cs \<tau> = beh)"
   by (meson assms functional_simulate_fin_complete functional_simulate_fin_sound)
 
-definition "functional_simulate maxtime cs = 
+definition "functional_simulate maxtime cs =
             Predicate.the (b_simulate_i_i_o maxtime cs)"
 
-theorem functional_simulate_complete:         
+theorem functional_simulate_complete:
   assumes "b_simulate maxtime cs beh"
   shows "functional_simulate maxtime cs = beh"
   using assms unfolding functional_simulate_def b_simulate_i_i_o_def
@@ -705,24 +712,40 @@ proof -
   have the_beh: "The (b_simulate maxtime cs) = beh"
     using assms unfolding functional_simulate_def b_simulate_i_i_o_def Predicate.the_def pred.sel
     by auto
-  have "\<theta> = add_to_beh def_state {} 0 0 t"
-    using assms(2) by (auto simp add: Let_def)
-  also have "... = override_lookups_on_open_right empty_trans (Some o def_state) 0 t"
-    unfolding add_to_beh_def by auto
-  finally have *: "\<forall>n\<ge>t. lookup \<theta> n = 0"
-    by transfer' auto
   have "t = next_time 0 \<tau>"
     using assms(2) by (auto simp add: Let_def)
   hence "\<forall>n. n < t \<longrightarrow> get_trans \<tau> n = 0"
     using next_time_at_least2 by auto
-  hence "\<forall>n<t. lookup \<tau> n = 0 "
+  hence look: "\<forall>n<t. lookup \<tau> n = 0 "
     by auto
-  hence **: "b_simulate_fin maxtime t \<sigma> \<gamma> \<theta> cs \<tau> (Poly_Mapping.update (maxtime + 1) 0 \<theta>')"
-    using small_step_implies_big_step[OF assms(3)] * by auto
-  have "b_simulate maxtime cs (Poly_Mapping.update (maxtime + 1) 0 \<theta>')"
-    using b_simulate.intros[OF assms(1) _ _ _ _ **] assms(2) by (auto simp add: Let_def)
+  have "0 < t \<or> t = 0" by auto
+  moreover
+  { assume "0 < t"
+    have "\<theta> = add_to_beh def_state {} 0 0 t"
+      using assms(2) by (auto simp add: Let_def)
+    also have "... = Poly_Mapping.update 0 (Some o def_state) empty_trans"
+      unfolding add_to_beh_def using `0 < t` by auto
+    finally have *: "\<forall>n\<ge>t. lookup \<theta> n = 0"
+      using `0 < t` by transfer' auto
+    hence **: "b_simulate_fin maxtime t \<sigma> \<gamma> \<theta> cs \<tau> (Poly_Mapping.update (maxtime + 1) 0 \<theta>')"
+      using small_step_implies_big_step[OF assms(3)] look by auto }
+  moreover
+  { assume "t = 0"
+    have "\<theta> = add_to_beh def_state {} 0 0 t"
+      using assms(2) by (auto simp add: Let_def)
+    also have "... = empty_trans"
+      unfolding add_to_beh_def using `t = 0` by auto
+    finally have *: "\<forall>n\<ge>t. lookup \<theta> n = 0"
+      by transfer auto
+    hence **: "b_simulate_fin maxtime t \<sigma> \<gamma> \<theta> cs \<tau> (Poly_Mapping.update (maxtime + 1) 0 \<theta>')"
+      using small_step_implies_big_step[OF assms(3)] look by auto }
+
+  ultimately have "b_simulate_fin maxtime t \<sigma> \<gamma> \<theta> cs \<tau> (Poly_Mapping.update (maxtime + 1) 0 \<theta>')"
+    by auto
+  hence "b_simulate maxtime cs (Poly_Mapping.update (maxtime + 1) 0 \<theta>')"
+    using b_simulate.intros[OF assms(1)] assms(2) by (auto simp add: Let_def)
   thus "b_simulate maxtime cs beh"
-    unfolding the_beh[THEN sym]   by (auto simp add: b_sim_init_deterministic intro: theI)
+    unfolding the_beh[THEN sym] by (auto simp add: b_sim_init_deterministic intro: theI)
 qed
 
 theorem
